intermediate/Veritas.Intermediate.Blum.fst
@@ -8,14 +8,14 @@ module SA = Veritas.SeqAux
 
 let rec add_seq_aux #vcfg (ils: its_log vcfg):
   Tot (seq ms_hashfn_dom)
-  (decreases (I.length ils)) = 
+  (decreases (I.length ils)) =
   let n = I.length ils in
   if n = 0 then S.empty #ms_hashfn_dom
   else
     let ils' = I.prefix ils (n - 1) in
     let s' = add_seq_aux ils' in
     let e = I.index ils (n - 1) in
-    if is_blum_add e then 
+    if is_blum_add e then
       append1 s' (IntT.blum_add_elem e)
     else
       s'
@@ -26,39 +26,39 @@ let add_seq = add_seq_aux
 
 /// map an index of ts containing a blum add to its position in the ts_add_seq
 ///  TODO: No idea why this proof is stressing out F*/Z3
-let rec add_seq_map 
+let rec add_seq_map
   #vcfg
-  (itsl: its_log vcfg) 
-  (i: I.seq_index itsl{is_blum_add (I.index itsl i)}): 
-  Tot (j:SA.seq_index (add_seq itsl){S.index (add_seq itsl) j = 
+  (itsl: its_log vcfg)
+  (i: I.seq_index itsl{is_blum_add (I.index itsl i)}):
+  Tot (j:SA.seq_index (add_seq itsl){S.index (add_seq itsl) j =
                                      blum_add_elem itsl i})
-  (decreases (I.length itsl)) =      
+  (decreases (I.length itsl)) =
   let n = I.length itsl in
   let s = add_seq itsl in
-  if n = 0 
-  then 0    
-  else 
+  if n = 0
+  then 0
+  else
     let itsl' = I.prefix itsl (n - 1) in
     let s' = add_seq itsl' in
     if i = n - 1 then S.length s'
-    else 
+    else
       //add_seq_map itsl' i
       let e = I.index itsl (n - 1) in
       if is_blum_add e then (
         // assert(add_seq itsl == append1 s' (IntT.blum_add_elem e));
         add_seq_map itsl' i
       )
-      else 
-        add_seq_map itsl' i        
+      else
+        add_seq_map itsl' i
 
 #pop-options
 
 #push-options "--z3rlimit_factor 3"
 
 let rec add_seq_map_inv #vcfg (itsl: its_log vcfg) (j: SA.seq_index (add_seq itsl)):
-  Tot (i: I.seq_index itsl {is_blum_add (I.index itsl i) /\ 
+  Tot (i: I.seq_index itsl {is_blum_add (I.index itsl i) /\
                             add_seq_map itsl i = j})
-  (decreases (I.length itsl)) = 
+  (decreases (I.length itsl)) =
   let n = I.length itsl in
   let s = add_seq itsl in
   if n = 0 then 0
@@ -69,42 +69,46 @@ let rec add_seq_map_inv #vcfg (itsl: its_log vcfg) (j: SA.seq_index (add_seq its
     if is_blum_add e then (
       assert(s == SA.append1 s' (IntT.blum_add_elem e));
       if j = S.length s' then n - 1
-      else add_seq_map_inv itsl' j        
+      else add_seq_map_inv itsl' j
     )
-    else add_seq_map_inv itsl' j 
+    else add_seq_map_inv itsl' j
   )
 
 #pop-options
 
+#push-options "--max_fuel 1 --max_ifuel 0 --z3rlimit_factor 3"
+
 let rec lemma_add_seq_map_inv #vcfg (itsl: its_log vcfg) (i: I.seq_index itsl{is_blum_add (I.index itsl i)}):
   Lemma (ensures (add_seq_map_inv itsl (add_seq_map itsl i) = i))
         (decreases (I.length itsl))
-        [SMTPat (add_seq_map itsl i)] = 
+        [SMTPat (add_seq_map itsl i)] =
   let n = I.length itsl in
   let s = add_seq itsl in
   if n = 0 then ()
-  else 
+  else
     let itsl' = I.prefix itsl (n - 1) in
     let s' = add_seq itsl' in
     if i = n - 1 then ()
-    else 
-      lemma_add_seq_map_inv itsl' i  
+    else
+      lemma_add_seq_map_inv itsl' i
+
+#pop-options
 
 let lemma_add_elem_correct (#vcfg:_) (itsl: its_log vcfg) (i: I.seq_index itsl):
   Lemma (requires (is_blum_add (I.index itsl i)))
         (ensures (add_set itsl `contains` blum_add_elem itsl i)) =
-  let sa = add_seq itsl in        
+  let sa = add_seq itsl in
   let j = add_seq_map itsl i in
   //assert(S.index sa j = blum_add_elem (I.index itsl i));
-  mset_contains_seq_element #_ #ms_hashfn_dom_cmp sa j    
+  mset_contains_seq_element #_ #ms_hashfn_dom_cmp sa j
 
 /// into mapping from ts add seq to global add seq
 let global_to_ts_addset_map_aux #vcfg (itsl: its_log vcfg) (i: SA.seq_index (IntG.add_seq (g_logS_of itsl))):
-  Tot (j: SA.seq_index (add_seq itsl) 
+  Tot (j: SA.seq_index (add_seq itsl)
        {
-          S.index (IntG.add_seq (g_logS_of itsl)) i = 
+          S.index (IntG.add_seq (g_logS_of itsl)) i =
           S.index (add_seq itsl) j
-       }) =          
+       }) =
   let gl = g_logS_of itsl in
   let gs = IntG.add_seq gl in
   let ii = IntG.add_set_map_inv gl i in
@@ -118,34 +122,34 @@ open FStar.Classical
 let lemma_global_to_ts_addset_map_into #vcfg (itsl: its_log vcfg):
   Lemma (forall (i1: SA.seq_index (IntG.add_seq (g_logS_of itsl))).
          forall (i2: SA.seq_index (IntG.add_seq (g_logS_of itsl))).
-         i1 <> i2 ==> global_to_ts_addset_map_aux itsl i1 <> 
-                    global_to_ts_addset_map_aux itsl i2) = 
+         i1 <> i2 ==> global_to_ts_addset_map_aux itsl i1 <>
+                    global_to_ts_addset_map_aux itsl i2) =
   let gl = g_logS_of itsl in
   let gs = IntG.add_seq gl in
-  
+
   let aux (i1 i2: SA.seq_index gs):
     Lemma (requires True)
           (ensures (i1 <> i2 ==> global_to_ts_addset_map_aux itsl i1 <>
-                               global_to_ts_addset_map_aux itsl i2)) = ()    
-  in  
+                               global_to_ts_addset_map_aux itsl i2)) = ()
+  in
   forall_intro_2 aux
 
 let global_to_ts_addset_map #vcfg (itsl: its_log vcfg):
-  into_smap (IntG.add_seq (g_logS_of itsl)) 
-       (add_seq itsl) = 
+  into_smap (IntG.add_seq (g_logS_of itsl))
+       (add_seq itsl) =
   lemma_global_to_ts_addset_map_into itsl;
   global_to_ts_addset_map_aux itsl
 
 let ts_to_global_addset_map_aux #vcfg (itsl: its_log vcfg) (j: SA.seq_index (add_seq itsl)):
   Tot (i: SA.seq_index (IntG.add_seq (g_logS_of itsl))
        {
-          S.index (IntG.add_seq (g_logS_of itsl)) i = 
+          S.index (IntG.add_seq (g_logS_of itsl)) i =
           S.index (add_seq itsl) j
-       }) = 
+       }) =
  let gl = g_logS_of itsl in
  let gs = IntG.add_seq gl in
  let ts = add_seq itsl in
- let i' = add_seq_map_inv itsl j in  
+ let i' = add_seq_map_inv itsl j in
  let ii = i2s_map itsl i' in
  let i = IntG.add_set_map gl ii in
  i
@@ -154,7 +158,7 @@ let lemma_ts_to_global_addset_map_into #vcfg (itsl: its_log vcfg):
   Lemma (forall (i1: SA.seq_index (add_seq itsl)).
          forall (i2: SA.seq_index (add_seq itsl)).
            i1 <> i2 ==> ts_to_global_addset_map_aux itsl i1 <>
-                      ts_to_global_addset_map_aux itsl i2) = 
+                      ts_to_global_addset_map_aux itsl i2) =
   let gl = g_logS_of itsl in
   let gs = IntG.add_seq gl in
   let ts = add_seq itsl in
@@ -167,17 +171,17 @@ let lemma_ts_to_global_addset_map_into #vcfg (itsl: its_log vcfg):
 
 let ts_to_global_addset_map #vcfg (itsl: its_log vcfg):
   into_smap (add_seq itsl)
-            (IntG.add_seq (g_logS_of itsl)) = 
+            (IntG.add_seq (g_logS_of itsl)) =
   lemma_ts_to_global_addset_map_into itsl;
   ts_to_global_addset_map_aux itsl
 
 
-let lemma_add_set_correct (#vcfg:_) (itsl: its_log vcfg): 
-  Lemma (ensures (add_set itsl == IntG.add_set (g_logS_of itsl))) = 
+let lemma_add_set_correct (#vcfg:_) (itsl: its_log vcfg):
+  Lemma (ensures (add_set itsl == IntG.add_set (g_logS_of itsl))) =
   let gl = g_logS_of itsl in
   let gs = IntG.add_seq gl in
   let ts = add_seq itsl in
-  
+
   bijection_seq_mset #_ #ms_hashfn_dom_cmp gs ts (global_to_ts_addset_map itsl)
                              (ts_to_global_addset_map itsl);
   ()
@@ -188,23 +192,23 @@ let lemma_add_set_extend  (#vcfg:_) (itsl: its_log vcfg {I.length itsl > 0}):
                   let e = I.index itsl i in
                   let be = blum_add_elem itsl i in
                   let itsl' = I.prefix itsl i in
-                  add_set itsl == 
-                  add_elem (add_set itsl') be)) = 
+                  add_set itsl ==
+                  add_elem (add_set itsl') be)) =
   let n = I.length itsl in
   let e = I.telem itsl in
   let itsl' = I.prefix itsl (n - 1) in
   let s' = add_seq itsl' in
   let be = IntT.blum_add_elem e in
-  seq2mset_add_elem #_ #ms_hashfn_dom_cmp s' be                  
+  seq2mset_add_elem #_ #ms_hashfn_dom_cmp s' be
 
 let lemma_blum_evict_elem (#vcfg:_) (itsl: its_log vcfg) (i:nat{i <= I.length itsl}) (j:nat{j < i})
   : Lemma (requires (is_evict_to_blum (I.index itsl j)))
-          (ensures (blum_evict_elem itsl j = blum_evict_elem (I.prefix itsl i) j)) = 
+          (ensures (blum_evict_elem itsl j = blum_evict_elem (I.prefix itsl i) j)) =
   let gl = g_logS_of itsl in
   let (t,j') = i2s_map itsl j in
-  let tl = thread_log gl t in  
+  let tl = thread_log gl t in
   assert(blum_evict_elem itsl j = IntT.blum_evict_elem tl j');
-  
+
   let itsl' = I.prefix itsl i in
   let gl' = g_logS_of itsl' in
   let tl' = thread_log gl' t in
@@ -215,9 +219,9 @@ let lemma_blum_evict_elem (#vcfg:_) (itsl: its_log vcfg) (i:nat{i <= I.length it
   //assert(tl' = VT.prefix tl (VT.length tl'));
   lemma_blum_evict_elem_prefix tl (IntT.length tl') j'
 
-let rec evict_seq_aux #vcfg (itsl: its_log vcfg): 
+let rec evict_seq_aux #vcfg (itsl: its_log vcfg):
   Tot (seq ms_hashfn_dom)
-  (decreases (I.length itsl)) = 
+  (decreases (I.length itsl)) =
   let n = I.length itsl in
   if n = 0 then S.empty #ms_hashfn_dom
   else
@@ -235,30 +239,30 @@ let evict_seq (#vcfg:_) (itsl: its_log vcfg): seq ms_hashfn_dom =
 #push-options "--z3rlimit_factor 3"
 
 let rec evict_seq_map #vcfg (itsl: its_log vcfg) (i:I.seq_index itsl {is_evict_to_blum (I.index itsl i)}):
-  Tot (j:SA.seq_index (evict_seq itsl){S.index (evict_seq itsl) j = 
-                                          blum_evict_elem itsl i}) 
-  (decreases (I.length itsl)) = 
+  Tot (j:SA.seq_index (evict_seq itsl){S.index (evict_seq itsl) j =
+                                          blum_evict_elem itsl i})
+  (decreases (I.length itsl)) =
   let n = I.length itsl in
   let itsl' = I.prefix itsl (n - 1) in
   let s' = evict_seq itsl' in
   if i = n - 1 then S.length s'
-  else ( 
+  else (
     lemma_blum_evict_elem itsl (n - 1) i;
     let e = I.index itsl (n - 1) in
-    if is_evict_to_blum e then 
+    if is_evict_to_blum e then
       evict_seq_map itsl' i
-    
-    else 
+
+    else
       evict_seq_map itsl' i
-    
+
   )
-  
+
 #pop-options
 
 let rec evict_seq_inv_map #vcfg (itsl: its_log vcfg) (j:SA.seq_index (evict_seq itsl)):
   Tot (i:I.seq_index itsl {is_evict_to_blum (I.index itsl i) /\
-                           evict_seq_map itsl i = j}) 
-  (decreases (I.length itsl)) = 
+                           evict_seq_map itsl i = j})
+  (decreases (I.length itsl)) =
   let n = I.length itsl in
   let itsl' = I.prefix itsl (n - 1) in
   let s' = evict_seq itsl' in
@@ -272,12 +276,12 @@ let rec evict_seq_inv_map #vcfg (itsl: its_log vcfg) (j:SA.seq_index (evict_seq 
 let rec lemma_evict_seq_inv_map #vcfg (itsl: its_log vcfg) (i:I.seq_index itsl {is_evict_to_blum (I.index itsl i)}):
   Lemma (ensures (evict_seq_inv_map itsl (evict_seq_map itsl i) = i))
         (decreases (I.length itsl))
-        [SMTPat (evict_seq_map itsl i)] = 
+        [SMTPat (evict_seq_map itsl i)] =
   let n = I.length itsl in
   let itsl' = I.prefix itsl (n - 1) in
   let s' = evict_seq itsl' in
   if i = n - 1 then ()
-  else 
+  else
     lemma_evict_seq_inv_map itsl' i
 #pop-options
 
@@ -286,7 +290,7 @@ let global_to_ts_evictseq_map_aux #vcfg (itsl: its_log vcfg) (i: SA.seq_index (I
        {
          S.index (IntG.evict_seq (g_logS_of itsl)) i =
          S.index (evict_seq itsl) j
-       }) = 
+       }) =
   let gl = g_logS_of itsl in
   let gs = IntG.evict_seq gl in
   let ii = IntG.evict_seq_map_inv gl i in
@@ -299,19 +303,19 @@ let lemma_global_to_ts_evictseq_map_into #vcfg (itsl: its_log vcfg):
   Lemma (forall (i1: SA.seq_index (IntG.evict_seq (g_logS_of itsl))).
          forall (i2: SA.seq_index (IntG.evict_seq (g_logS_of itsl))).
          i1 <> i2 ==> global_to_ts_evictseq_map_aux itsl i1 <>
-                    global_to_ts_evictseq_map_aux itsl i2) = 
+                    global_to_ts_evictseq_map_aux itsl i2) =
   let gl = g_logS_of itsl in
   let gs = IntG.evict_seq gl in
   let aux (i1 i2: SA.seq_index gs):
     Lemma (requires True)
           (ensures (i1 <> i2 ==> global_to_ts_evictseq_map_aux itsl i1 <>
-                               global_to_ts_evictseq_map_aux itsl i2)) = ()    
-  in  
-  forall_intro_2 aux                   
+                               global_to_ts_evictseq_map_aux itsl i2)) = ()
+  in
+  forall_intro_2 aux
 
 let global_to_ts_evictseq_map #vcfg (itsl: its_log vcfg):
   into_smap (IntG.evict_seq (g_logS_of itsl))
-            (evict_seq itsl) = 
+            (evict_seq itsl) =
   lemma_global_to_ts_evictseq_map_into itsl;
   global_to_ts_evictseq_map_aux itsl
 
@@ -320,8 +324,8 @@ let ts_to_global_evictseq_map_aux #vcfg (itsl: its_log vcfg) (j:SA.seq_index (ev
        {
          S.index (IntG.evict_seq (g_logS_of itsl)) i =
          S.index (evict_seq itsl) j
-       }) = 
-  let gl = g_logS_of itsl in       
+       }) =
+  let gl = g_logS_of itsl in
   let gs = IntG.evict_seq gl in
   let ts = evict_seq itsl in
   let i' = evict_seq_inv_map itsl j in
@@ -333,61 +337,61 @@ let lemma_ts_to_global_evictseq_map_into #vcfg (itsl: its_log vcfg):
   Lemma (forall (i1: SA.seq_index (evict_seq itsl)).
          forall (i2: SA.seq_index (evict_seq itsl)).
          i1 <> i2 ==> ts_to_global_evictseq_map_aux itsl i1 <>
-                    ts_to_global_evictseq_map_aux itsl i2) = 
+                    ts_to_global_evictseq_map_aux itsl i2) =
   let ts = evict_seq itsl in
 
   let aux (i1 i2: SA.seq_index ts):
     Lemma (i1 <> i2 ==> ts_to_global_evictseq_map_aux itsl i1 <>
                       ts_to_global_evictseq_map_aux itsl i2) = ()
-  in                      
+  in
   forall_intro_2 aux
 
 let ts_to_global_evictseq_map #vcfg (itsl: its_log vcfg):
   into_smap (evict_seq itsl)
-            (IntG.evict_seq (g_logS_of itsl)) = 
+            (IntG.evict_seq (g_logS_of itsl)) =
   lemma_ts_to_global_evictseq_map_into itsl;
   ts_to_global_evictseq_map_aux itsl
 
 let evict_set_correct (#vcfg:_) (itsl: its_log vcfg):
-  Lemma (ensures (evict_set itsl == IntG.evict_set (g_logS_of itsl))) = 
+  Lemma (ensures (evict_set itsl == IntG.evict_set (g_logS_of itsl))) =
   let gl = g_logS_of itsl in
   let gs = IntG.evict_seq gl in
   let ts = evict_seq itsl in
-  
+
   bijection_seq_mset #_ #ms_hashfn_dom_cmp gs ts (global_to_ts_evictseq_map itsl)
                              (ts_to_global_evictseq_map itsl)
 
 let lemma_evict_elem_correct (#vcfg:_) (itsl: its_log vcfg) (i: I.seq_index itsl):
   Lemma (requires (is_evict_to_blum (I.index itsl i)))
-        (ensures (evict_set itsl `contains` blum_evict_elem itsl i)) = 
-  let es = evict_seq itsl in        
+        (ensures (evict_set itsl `contains` blum_evict_elem itsl i)) =
+  let es = evict_seq itsl in
   let j = evict_seq_map itsl i in
   mset_contains_seq_element #_ #ms_hashfn_dom_cmp es j
 
 let lemma_evict_set_extend2 (#vcfg:_) (itsl: its_log vcfg{I.length itsl > 0}):
-  Lemma (requires (let i = I.length itsl - 1 in  
+  Lemma (requires (let i = I.length itsl - 1 in
                    not (is_evict_to_blum (I.index itsl i))))
-        (ensures (let i = I.length itsl - 1 in  
+        (ensures (let i = I.length itsl - 1 in
                   evict_set itsl == evict_set (I.prefix itsl i))) = ()
 
-let lemma_spec_rel_implies_same_add_elem (#vcfg:_) 
-                                         (ils: its_log vcfg{spec_rel ils}) 
+let lemma_spec_rel_implies_same_add_elem (#vcfg:_)
+                                         (ils: its_log vcfg{spec_rel ils})
                                          (i: I.seq_index ils{is_blum_add (I.index ils i)}):
   Lemma (ensures (let ilk = IntTS.to_logk ils in
                   SpecV.is_blum_add (I.index ilk i) /\
-                  SpecT.blum_add_elem (I.index ilk i) = blum_add_elem ils i)) =   
+                  SpecT.blum_add_elem (I.index ilk i) = blum_add_elem ils i)) =
   ()
 
 let rec lemma_spec_rel_implies_same_add_seq_len #vcfg (ils: its_log vcfg{spec_rel ils})
   : Lemma (ensures (let ilk = to_logk ils in
-                    S.length (add_seq ils) = S.length (SpecB.ts_add_seq ilk))) 
-          (decreases (I.length ils)) =   
-  let ilk = to_logk ils in                    
+                    S.length (add_seq ils) = S.length (SpecB.ts_add_seq ilk)))
+          (decreases (I.length ils)) =
+  let ilk = to_logk ils in
   let as_s = add_seq ils in
   let as_k = SpecB.ts_add_seq ilk in
-  let n = I.length ils in 
-  if n = 0 then 
-    SpecB.lemma_add_seq_empty ilk  
+  let n = I.length ils in
+  if n = 0 then
+    SpecB.lemma_add_seq_empty ilk
   else (
     let ils' = I.prefix ils (n - 1) in
     let ilk' = to_logk ils' in
@@ -401,18 +405,18 @@ let rec lemma_spec_rel_implies_same_add_seq_len #vcfg (ils: its_log vcfg{spec_re
 
     if is_blum_add es then
       // assert(SpecV.is_blum_add ek);
-      SpecB.lemma_add_seq_extend ilk    
-    else      
-      SpecB.lemma_add_seq_extend2 ilk     
+      SpecB.lemma_add_seq_extend ilk
+    else
+      SpecB.lemma_add_seq_extend2 ilk
   )
 
 let rec lemma_spec_rel_implies_same_add_seq_aux (#vcfg:_) (ils: its_log vcfg{spec_rel ils})
-  : Lemma (ensures (let ilk = to_logk ils in 
+  : Lemma (ensures (let ilk = to_logk ils in
                     add_seq ils = SpecB.ts_add_seq ilk))
-          (decreases (I.length ils)) =                     
+          (decreases (I.length ils)) =
   let ilk = to_logk ils in
   let asl = add_seq ils in
-  let ask = SpecB.ts_add_seq ilk in  
+  let ask = SpecB.ts_add_seq ilk in
   let n = I.length ils in
   if n = 0 then (
     SpecB.lemma_add_seq_empty ilk;
@@ -431,25 +435,25 @@ let rec lemma_spec_rel_implies_same_add_seq_aux (#vcfg:_) (ils: its_log vcfg{spe
     lemma_spec_rel_implies_same_add_seq_aux ils';
     if is_blum_add es then
       // assert(SpecV.is_blum_add ek);
-      SpecB.lemma_add_seq_extend ilk    
-    else      
-      SpecB.lemma_add_seq_extend2 ilk       
+      SpecB.lemma_add_seq_extend ilk
+    else
+      SpecB.lemma_add_seq_extend2 ilk
   )
 
 let lemma_spec_rel_implies_same_add_seq (#vcfg:_) (ils: its_log vcfg{spec_rel ils})
-  : Lemma (ensures (let ilk = to_logk ils in 
-                    add_seq ils = SpecB.ts_add_seq ilk)) = 
+  : Lemma (ensures (let ilk = to_logk ils in
+                    add_seq ils = SpecB.ts_add_seq ilk)) =
   lemma_spec_rel_implies_same_add_seq_aux ils
 
 module SpecTS = Veritas.Verifier.TSLog
 
-let lemma_spec_rel_implies_same_evict_elem (#vcfg:_) 
-                                         (ils: its_log vcfg{spec_rel ils}) 
+let lemma_spec_rel_implies_same_evict_elem (#vcfg:_)
+                                         (ils: its_log vcfg{spec_rel ils})
                                          (i: I.seq_index ils{is_evict_to_blum (I.index ils i)}):
   Lemma (ensures (let ilk = IntTS.to_logk ils in
                   SpecV.is_evict_to_blum (I.index ilk i) /\
-                  SpecB.blum_evict_elem ilk i = blum_evict_elem ils i)) = 
-  let ilk = IntTS.to_logk ils in                  
+                  SpecB.blum_evict_elem ilk i = blum_evict_elem ils i)) =
+  let ilk = IntTS.to_logk ils in
   // let bes = blum_evict_elem ils i in
   // let bek = SpecB.blum_evict_elem ilk i in
   // let tid = IntTS.thread_id_of ils i in
@@ -465,7 +469,7 @@ let lemma_spec_rel_implies_same_evict_elem (#vcfg:_)
   SpecTS.lemma_blum_evict_def ilk i;
 
   // let s = slot_of es in
-  // assert(inuse_slot sts s); 
+  // assert(inuse_slot sts s);
   // let k = stored_key sts s in
   // assert(SpecV.key_of ek = k);
 
@@ -475,13 +479,13 @@ let lemma_spec_rel_implies_same_evict_elem (#vcfg:_)
   assert(vtls_rel vss vsk);
   // assert(SpecV.store_contains stk k);
   // assert(SpecV.stored_value stk k = v);
-  ()                  
+  ()
 
 let rec lemma_spec_rel_implies_same_evict_seq_aux (#vcfg:_) (ils: its_log vcfg{spec_rel ils})
-  : Lemma (ensures (let ilk = to_logk ils in 
+  : Lemma (ensures (let ilk = to_logk ils in
                     evict_seq ils = SpecB.ts_evict_seq ilk))
           (decreases (I.length ils))
-  = 
+  =
   let ilk = to_logk ils in
   let esl = evict_seq ils in
   let esk = SpecB.ts_evict_seq ilk in
@@ -494,7 +498,7 @@ let rec lemma_spec_rel_implies_same_evict_seq_aux (#vcfg:_) (ils: its_log vcfg{s
   else (
     let ils' = I.prefix ils (n - 1) in
     let ilk' = to_logk ils' in
-    let es = I.index ils (n - 1) in 
+    let es = I.index ils (n - 1) in
     let ek = I.index ilk (n - 1) in
     lemma_spec_rel_implies_prefix_spec_rel ils (n -1);
     lemma_spec_rel_implies_same_evict_seq_aux ils';
@@ -502,21 +506,21 @@ let rec lemma_spec_rel_implies_same_evict_seq_aux (#vcfg:_) (ils: its_log vcfg{s
       SpecB.lemma_evict_seq_extend ilk;
       lemma_spec_rel_implies_same_evict_elem ils (n - 1)
     )
-    else 
-      SpecB.lemma_evict_seq_extend2 ilk    
+    else
+      SpecB.lemma_evict_seq_extend2 ilk
   )
 
 
 let lemma_spec_rel_implies_same_evict_seq (#vcfg:_) (ils: its_log vcfg{spec_rel ils})
-  : Lemma (ensures (let ilk = to_logk ils in 
+  : Lemma (ensures (let ilk = to_logk ils in
                     evict_seq ils = SpecB.ts_evict_seq ilk))
   = lemma_spec_rel_implies_same_evict_seq_aux ils
 
-(* since evict_set is a pure set (not a multiset) we can identify the unique index 
+(* since evict_set is a pure set (not a multiset) we can identify the unique index
  * for each element of the set *)
 let index_blum_evict (#vcfg:_) (itsl: its_log vcfg) (e: ms_hashfn_dom {evict_set itsl `contains` e}):
-  (i:I.seq_index itsl{is_evict_to_blum (I.index itsl i) /\ 
-                      blum_evict_elem itsl i = e}) = 
+  (i:I.seq_index itsl{is_evict_to_blum (I.index itsl i) /\
+                      blum_evict_elem itsl i = e}) =
   let esq = evict_seq itsl in
   let est = evict_set itsl in
   let j = index_of_mselem #_ #ms_hashfn_dom_cmp esq e in
@@ -525,14 +529,14 @@ let index_blum_evict (#vcfg:_) (itsl: its_log vcfg) (e: ms_hashfn_dom {evict_set
 
 (* the clock of an evict entry is the timestamp in the corresponding blum element *)
 let lemma_evict_clock  #vcfg (itsl: its_log vcfg) (i:I.seq_index itsl{is_evict_to_blum (I.index itsl i)}):
-  Lemma (IntTS.clock itsl i = timestamp_of (blum_evict_elem itsl i)) = 
+  Lemma (IntTS.clock itsl i = timestamp_of (blum_evict_elem itsl i)) =
   let gl = g_logS_of itsl in
   let (tid,j) = i2s_map itsl i in
   let tl = thread_log gl tid in
   IntT.lemma_evict_clock tl j
 
 let lemma_add_clock #vcfg (itsl: its_log vcfg) (i: I.seq_index itsl{is_blum_add (I.index itsl i)}):
-  Lemma (timestamp_of (blum_add_elem itsl i) `ts_lt` IntTS.clock itsl i) = 
+  Lemma (timestamp_of (blum_add_elem itsl i) `ts_lt` IntTS.clock itsl i) =
   let gl = g_logS_of itsl in
   let (tid,j) = i2s_map itsl i in
   let tl = thread_log gl tid in
@@ -541,29 +545,29 @@ let lemma_add_clock #vcfg (itsl: its_log vcfg) (i: I.seq_index itsl{is_blum_add 
 (* if the blum add occurs in the blum evict set, its index is earlier *)
 let lemma_evict_before_add (#vcfg:_) (itsl: its_log vcfg) (i:I.seq_index itsl{is_blum_add (I.index itsl i)}):
   Lemma (ensures (not (evict_set itsl `contains` blum_add_elem itsl i)) \/
-                  index_blum_evict itsl (blum_add_elem itsl i) < i) = 
-  let be = blum_add_elem itsl i in                  
+                  index_blum_evict itsl (blum_add_elem itsl i) < i) =
+  let be = blum_add_elem itsl i in
   let evt_set = evict_set itsl in
   let add_set = add_set itsl in
   lemma_add_clock itsl i;
   if evt_set `contains` be then (
     let j = index_blum_evict itsl be in
-    lemma_evict_clock itsl j;    
-    lemma_clock_ordering itsl j i    
+    lemma_evict_clock itsl j;
+    lemma_clock_ordering itsl j i
   )
   else ()
 
-let some_add_elem_idx (#vcfg:_) (itsl: its_log vcfg) 
+let some_add_elem_idx (#vcfg:_) (itsl: its_log vcfg)
                                 (be: ms_hashfn_dom{add_set itsl `contains` be}):
-   (i:(I.seq_index itsl){is_blum_add (I.index itsl i) /\ be = blum_add_elem itsl i}) = 
-  let s = add_seq itsl in  
+   (i:(I.seq_index itsl){is_blum_add (I.index itsl i) /\ be = blum_add_elem itsl i}) =
+  let s = add_seq itsl in
   (* index of element be in s *)
   let j = index_of_mselem #_ #ms_hashfn_dom_cmp s be in
   add_seq_map_inv itsl j
 
 let rec lemma_prefix_add_seq #vcfg (itsl: its_log vcfg) (i: nat{ i <= I.length itsl}):
   Lemma (ensures (SA.is_prefix (add_seq itsl) (add_seq (I.prefix itsl i))))
-        (decreases (I.length itsl)) = 
+        (decreases (I.length itsl)) =
   let n = I.length itsl in
   if i = n then () // prefix is the same sequence
   else (
@@ -583,7 +587,7 @@ let rec lemma_prefix_add_seq #vcfg (itsl: its_log vcfg) (i: nat{ i <= I.length i
   )
 
 let lemma_mem_monotonic_add_set (#vcfg:_) (be:ms_hashfn_dom) (itsl: its_log vcfg) (i:nat{i <= I.length itsl}):
-  Lemma (mem be (add_set itsl) >= mem be (add_set (I.prefix itsl i))) = 
+  Lemma (mem be (add_set itsl) >= mem be (add_set (I.prefix itsl i))) =
   let itsl' = I.prefix itsl i in
   let s' = add_seq itsl' in
   let s = add_seq itsl in
@@ -597,7 +601,7 @@ let lemma_add_delta_implies_not_eq (#vcfg:_) (itsl: its_log vcfg) (i:nat{i <= I.
     Lemma (requires (let itsli = I.prefix itsl i in
                      MS.mem be (add_set itsli) > MS.mem be (evict_set itsli)))
           (ensures (~ ((add_set itsl) == (evict_set itsl)))) =
-  let gl = g_logS_of itsl in      
+  let gl = g_logS_of itsl in
   let itsli = I.prefix itsl i in
   let asi = add_set itsli in
   let esi = evict_set itsli in
@@ -606,7 +610,7 @@ let lemma_add_delta_implies_not_eq (#vcfg:_) (itsl: its_log vcfg) (i:nat{i <= I.
 
   let j = some_add_elem_idx itsli be in
   lemma_mem_monotonic_add_set be itsl i;
-  
+
   if es `contains` be then (
     lemma_evict_before_add itsl j;
     let j' = index_blum_evict itsl be in
